src/Rec.v
@@ -4,7 +4,7 @@ Require Import Eqdep_dec.
 Require Import Array.
 Require Import Psatz.
 Require Import ProofIrrelevance.
-
+Require Import ListUtils.
 Import ListNotations.
 Open Scope string_scope.
 
